dist/Kuiper_AtomicReduce_F64.cu
@@ -1,0 +1,24 @@
+
+
+#include "Kuiper_AtomicReduce_F64.h"
+
+__global__
+
+void Kuiper_AtomicReduce_F64_kernel(double_t *a, double_t *r)
+{
+  size_t bid = blockIdx_x();
+  size_t bdim = blockDim_x();
+  atomic_add_f64(r, a[bid * bdim + threadIdx_x()]);
+}
+
+double_t Kuiper_AtomicReduce_F64_reduce(size_t n, double_t *a)
+{
+  double_t r = (double_t)0.0l;
+  double_t *gr = (double_t *)KPR_GPU_ALLOC((size_t)8U);
+  MUST(cudaMemcpy(gr, &r, (size_t)8U, cudaMemcpyHostToDevice));
+  KPR_KCALL(Kuiper_AtomicReduce_F64_kernel, n, 1U, a, gr);
+  MUST(cudaMemcpy(&r, gr, (size_t)8U, cudaMemcpyDeviceToHost));
+  MUST(cudaFree(gr));
+  return r;
+}
+
