dist/Kuiper_AtomicReduce_U32.cu
@@ -1,0 +1,24 @@
+
+
+#include "Kuiper_AtomicReduce_U32.h"
+
+__global__
+
+void Kuiper_AtomicReduce_U32_kernel(uint32_t *a, uint32_t *r)
+{
+  size_t bid = blockIdx_x();
+  size_t bdim = blockDim_x();
+  atomic_add_u32(r, a[bid * bdim + threadIdx_x()]);
+}
+
+uint32_t Kuiper_AtomicReduce_U32_reduce(size_t n, uint32_t *a)
+{
+  uint32_t r = 0U;
+  uint32_t *gr = (uint32_t *)KPR_GPU_ALLOC((size_t)4U);
+  MUST(cudaMemcpy(gr, &r, (size_t)4U, cudaMemcpyHostToDevice));
+  KPR_KCALL(Kuiper_AtomicReduce_U32_kernel, n, 1U, a, gr);
+  MUST(cudaMemcpy(&r, gr, (size_t)4U, cudaMemcpyDeviceToHost));
+  MUST(cudaFree(gr));
+  return r;
+}
+
