dist/Kuiper_AtomicReduce_U64.cu
@@ -1,22 +1,22 @@
 
 
-#include "Kuiper_AtomicReduce.h"
+#include "Kuiper_AtomicReduce_U64.h"
 
 __global__
 
-static void kernel(uint64_t *a, uint64_t *r)
+void Kuiper_AtomicReduce_U64_kernel(uint64_t *a, uint64_t *r)
 {
   size_t bid = blockIdx_x();
   size_t bdim = blockDim_x();
   atomic_add_u64(r, a[bid * bdim + threadIdx_x()]);
 }
 
-uint64_t Kuiper_AtomicReduce_reduce(size_t n, uint64_t *a)
+uint64_t Kuiper_AtomicReduce_U64_reduce(size_t n, uint64_t *a)
 {
   uint64_t r = 0ULL;
   uint64_t *gr = (uint64_t *)KPR_GPU_ALLOC((size_t)8U);
   MUST(cudaMemcpy(gr, &r, (size_t)8U, cudaMemcpyHostToDevice));
-  KPR_KCALL(kernel, n, 1U, a, gr);
+  KPR_KCALL(Kuiper_AtomicReduce_U64_kernel, n, 1U, a, gr);
   MUST(cudaMemcpy(&r, gr, (size_t)8U, cudaMemcpyDeviceToHost));
   MUST(cudaFree(gr));
   return r;
