src/examples/Kuiper.AtomicReduce.F32.fsti
@@ -1,0 +1,7 @@
+module Kuiper.AtomicReduce.F32
+
+#lang-pulse
+open Kuiper
+open Kuiper.AtomicReduce.Poly
+
+val reduce : reduce_ty f32
