src/examples/Kuiper.AtomicReduce.Poly.fsti
@@ -1,0 +1,35 @@
+module Kuiper.AtomicReduce.Poly
+
+(* Reducing an array with some given operation. *)
+
+#lang-pulse
+
+open Kuiper
+open Kuiper.Atomics
+open Kuiper.AtomicReduce.Poly.Kernel
+
+module SZ = FStar.SizeT
+
+unfold
+type reduce_ty
+  (et : Type0) {| scalar et |} {| d : has_atomic_add et |} =
+  (n : sz) ->
+  (a : gpu_array et n) ->
+  (#f : perm) ->
+  (#v_a : erased (seq et)) ->
+  stt et
+  (requires
+    cpu **
+    pure (f == 1.0R) **
+    gpu_pts_to_array a #f v_a **
+    pure (SZ.v n > 0 /\ SZ.v n <= 1024))
+  (ensures fun r ->
+    cpu **
+    gpu_pts_to_array a #f v_a **
+    pure (r == Kuiper.Seq.Common.seq_fold_left d.pure_op zero v_a))
+
+inline_for_extraction noextract
+val reduce
+  (#et : Type0) {| scalar et |} {| d : has_atomic_add et |}
+  (k : kernel_ty et #_ #_)
+  : reduce_ty et #_ #_
