src/examples/Kuiper.AtomicReduce.U64.fst
@@ -1,0 +1,11 @@
+module Kuiper.AtomicReduce.U64
+
+#lang-pulse
+open Kuiper
+open Kuiper.AtomicReduce.Poly
+open Kuiper.AtomicReduce.Poly.Kernel
+
+[@@CPrologue "__global__"]
+let kernel : kernel_ty u64 = kernel #u64
+
+let reduce : reduce_ty u64 = reduce kernel
