src/lib/kuiper/Kuiper.Atomics.fsti
@@ -1,0 +1,51 @@
+module Kuiper.Atomics
+
+#lang-pulse
+
+open FStar.Tactics.Typeclasses
+open FStar.Ghost
+open Pulse.Lib.Core
+open Pulse.Class.PtsTo
+open Kuiper.Base
+open Kuiper.Ref
+open Kuiper.IntAliases
+open Kuiper.AtomicOps
+
+inline_for_extraction
+class has_atomic_add (t:Type) = {
+  [@@@no_method]
+  pure_op : t -> t -> t;
+  atomic_add :
+    (r : gpu_ref t) ->
+    (i : t) ->
+    (#v0 : erased t) ->
+    stt_atomic t
+      emp_inames
+      (requires gpu ** (r |-> v0))
+      (ensures fun old ->
+        ensures gpu ** (r |-> pure_op i v0) ** pure (old == reveal v0));
+}
+
+inline_for_extraction
+instance has_atomic_add_u32 : has_atomic_add u32 = {
+  pure_op = FStar.UInt32.add_mod;
+  atomic_add = gpu_faa_u32;
+}
+
+inline_for_extraction
+instance has_atomic_add_u64 : has_atomic_add u64 = {
+  pure_op = FStar.UInt64.add_mod;
+  atomic_add = gpu_faa_u64;
+}
+
+inline_for_extraction
+instance has_atomic_add_f32 : has_atomic_add f32 = {
+  pure_op = Kuiper.Float32.add;
+  atomic_add = gpu_faa_f32;
+}
+
+inline_for_extraction
+instance has_atomic_add_f64 : has_atomic_add f64 = {
+  pure_op = Kuiper.Float64.add;
+  atomic_add = gpu_faa_f64;
+}
